checking progress...

theories/L6_PCPS/Heap/closure_conversion_correct.v
@@ -1,8 +1,8 @@
 From L6 Require Import cps cps_util set_util identifiers ctx Ensembles_util
-     List_util functions closure_conversion closure_conversion_util
-     closure_conversion_correct.
+     List_util functions tactics.
 
-From L6.Heap Require Import heap heap_defs heap_equiv space_sem cc_log_rel size_cps.
+From L6.Heap Require Import heap heap_defs heap_equiv space_sem cc_log_rel size_cps closure_conversion
+     closure_conversion_util.
 
 From Coq Require Import ZArith.Znumtheory Relations.Relations Arith.Wf_nat
                         Lists.List MSets.MSets MSets.MSetRBT Numbers.BinNums
@@ -22,66 +22,243 @@ Module ClosureConversionCorrect (H : Heap).
          Size.Compat Size.
   
   Variable clo_tag : cTag.
-
+  
   (** Invariant about the free variables *) 
-  Definition FV_inv (k : nat) (IP : GIInv) (P : GInv) (b : Inj)
+  Definition FV_inv (k j : nat) (IP : GIInv) (P : GInv) (b : Inj)
              (rho1 : env) (H1 : heap block) (rho2 : env) (H2 : heap block)
-             (Scope Funs : Ensemble var) (c : cTag) (Γ : var) (FVs : list var) : Prop :=
-    forall (x : var) N,
-      ~ In _ Scope x ->
-      ~ In _ Funs x -> 
-      nthN FVs N = Some x ->
-      exists (v : value) (vs : list value) (l : loc) (v' : value),
-        M.get x rho1 = Some v /\
-        M.get Γ rho2 = Some (Loc l) /\
-        get l H2 = Some (Constr c vs) /\
-        nthN vs N = Some v' /\
-        (forall j, Res (v, H1) ≺ ^ ( k ; j ; IP ; P ; b) Res (v', H2)).
+             (c : cTag) (Γ : var) (FVs : list var) : Prop :=
+    exists (v : value) (vs : list value) (l : loc),
+      M.get Γ rho2 = Some (Loc l) /\
+      get l H2 = Some (Constr c vs) /\
+      Forall2 (fun x v' => 
+                 exists v, M.get x rho1 = Some v /\
+                      Res (v, H1) ≺ ^ ( k ; j ; IP ; P ; b) Res (v', H2)) FVs vs.
   
   (** Invariant about the functions in the current function definition *)
-  Definition Fun_inv (k : nat) (IP : GIInv) (P : GInv) (b : Inj)
+  Definition Fun_inv (k j : nat) (IP : GIInv) (P : GInv) (b : Inj)
              (rho1 : env) (H1 : heap block) (rho2 : env) (H2 : heap block)
-             (Scope Funs : Ensemble var) (σ : var -> var) (c : cTag) (Γ : var)  : Prop :=
+             (Scope Funs : Ensemble var) (σ : var -> var)  : Prop :=
+    (* (exists f, f \in Funs) /\ *)
     forall (f : var),
-      ~ In _ Scope f ->
-      In var Funs f ->
-      exists l_clo (vf1 venv : value),
-        M.get f rho1 = Some (Loc l_clo) /\
-        ~ l_clo \in env_locs rho1 Scope /\
-        ~ Scope (σ f) /\
-        M.get (σ f) rho2 = Some vf1 /\
-        M.get Γ rho2 = Some venv /\
-        forall l_clo' vs,
-          get l_clo' H2 = Some (Constr c (vf1 :: venv :: vs)) ->
-          (forall j, (Res (Loc l_clo, H1)) ≺ ^ ( k ; j; IP ; P ; b {l_clo ~> l_clo'}) (Res (Loc l_clo', H2))).
+     In var Funs f ->
+      exists lf1 lf2,
+        M.get f rho1 = Some lf1 /\ 
+        M.get (σ f) rho2 = Some lf2 /\
+        Res (lf1, H1) ≺ ^ ( k ; j ; IP ; P ; b) Res (lf2, H2).
   
   (** Versions without the logical relation. Useful when we're only interested in other invariants. *)
   
   (** Invariant about the free variables *) 
   Definition FV_inv_weak (rho1 : env) (rho2 : env) (H2 : heap block)
-             (Scope Funs : Ensemble var) (c : cTag) (Γ : var) (FVs : list var) : Prop :=
-    forall (x : var) N ,
-      ~ In _ Scope x ->
-      ~ In _ Funs x -> 
-      nthN FVs N = Some x ->
-      exists v (vs : list value) (l : loc) (v' : value),
-        M.get x rho1 = Some v /\
-        M.get Γ rho2 = Some (Loc l) /\
-        get l H2 = Some (Constr c vs) /\
-        nthN vs N = Some v'.
+             (c : cTag) (Γ : var) (FVs : list var) : Prop :=
+    exists (v : value) (vs : list value) (l : loc),
+      M.get Γ rho2 = Some (Loc l) /\
+      get l H2 = Some (Constr c vs) /\
+      Forall2 (fun x v' => exists v, M.get x rho1 = Some v) FVs vs.
   
   (** Invariant about the functions in the current function definition *)
-  Definition Fun_inv_weak (rho1 : env)  (rho2 : env)
-             (Scope Funs : Ensemble var) (σ : var -> var) (c : cTag) (Γ : var)  : Prop :=
-    forall (f : var) (vf1 : value),
-      ~ In _ Scope f ->
+  Definition Fun_inv_weak (rho1 : env) (H1 : heap block) (rho2 : env) (H2 : heap block)
+             (Scope Funs : Ensemble var) (σ : var -> var) : Prop :=
+    (* (exists f, f \in Funs \\ Scope) /\ *)
+    forall (f : var),
       In var Funs f ->
-      M.get f rho1 = Some vf1 ->
-      exists (vf1 venv : value),
-        ~ In _ Scope (σ f) /\
-        M.get (σ f) rho2 = Some vf1 /\
-        M.get Γ rho2 = Some venv.
+      exists lf1 lf2,
+        M.get f rho1 = Some lf1 /\ 
+        M.get (σ f) rho2 = Some lf2.
   
+  (** * Lemmas about [V_inv] *)
+
+  Lemma FV_inv_image_post (k j : nat) (GII : GIInv) (GI : GInv) (b : Inj)
+             (rho1 : env) (H1 : heap block) (rho2 : env) (H2 : heap block)
+             (c : cTag) (Γ : var) (FVs : list var) :
+    FV_inv k j GII GI b rho1 H1 rho2 H2 c Γ FVs ->    
+    image b ((post H1 ^ j) (env_locs rho1 (FromList FVs))) <-->
+    (post H2 ^ j) (post H2 (env_locs rho2 ([set Γ]))).
+  Proof.
+    intros Hfv. destruct Hfv as (v & vs & l & Hget1 & Hget2 & Hall).
+    rewrite (proper_post_n H2); [| now rewrite env_locs_Singleton; eauto; apply post_Singleton; eauto ].
+    simpl. clear Hget1 Hget2. induction Hall.
+    - simpl. rewrite post_n_Empty_set.
+      eapply Same_set_trans; [| eapply image_Empty_set with (g := b) ].
+      rewrite proper_post_n; [| rewrite FromList_nil, env_locs_Empty_set; reflexivity ].
+      rewrite post_n_Empty_set. reflexivity.
+    - rewrite proper_post_n; [| rewrite FromList_cons, env_locs_Union; reflexivity ].
+      simpl. rewrite !post_n_Union, image_Union.
+      eapply Same_set_Union_compat; [| now eauto ].
+      destruct H as [v' [Hget' Hres]].
+      rewrite proper_post_n; [| now eapply env_locs_Singleton; eauto ].
+      eapply cc_approx_val_image_eq. eassumption.
+  Qed.
+
+  Lemma FV_inv_j_monotonic (k j' j : nat) (GII : GIInv) (GI : GInv) (b : Inj)
+        (rho1 : env) (H1 : heap block) (rho2 : env) (H2 : heap block)
+        (c : cTag) (Γ : var) (FVs : list var) :
+    FV_inv k j GII GI b rho1 H1 rho2 H2 c Γ FVs ->
+    j' <= j ->
+    FV_inv k j' GII GI b rho1 H1 rho2 H2 c Γ FVs.
+  Proof.
+    intros Hfv Hlt. 
+    destruct Hfv as (v & vs & l & Hget1 & Hget2 & Hall).
+    repeat eexists; eauto.
+    eapply Forall2_monotonic; [| eassumption ].
+    intros x1 x2 [v' [Hget Hres]]. eexists; split; eauto.
+    eapply cc_approx_val_j_monotonic; eauto.
+  Qed.
+
+    
+  Lemma FV_inv_image_reach_n (k j : nat) (GII : GIInv) (GI : GInv) (b : Inj)
+             (rho1 : env) (H1 : heap block) (rho2 : env) (H2 : heap block)
+             (c : cTag) (Γ : var) (FVs : list var) :
+    FV_inv k j GII GI b rho1 H1 rho2 H2 c Γ FVs ->    
+    image b (reach_n H1 j (env_locs rho1 (FromList FVs))) <-->
+    (reach_n H2 j (post H2 (env_locs rho2 ([set Γ])))).
+  Proof.
+    intros Hfv. split.
+    - intros l' [l [[m [Hm Hr]] Hin]].
+      eapply FV_inv_j_monotonic in Hfv; eauto.
+      eexists m. split; eauto. eapply FV_inv_image_post. eassumption.
+      eexists; split; eauto.
+    - intros l' [m [Hm Hr]].
+      eapply FV_inv_j_monotonic in Hfv; eauto.
+      eapply FV_inv_image_post in Hr; eauto.
+      destruct Hr as [l [Heql Hin]]. eexists; split; eauto.
+      eexists; split; eauto.
+  Qed.
+
+  Lemma FV_inv_image_reach (k : nat) (GII : GIInv) (GI : GInv) (b : Inj)
+             (rho1 : env) (H1 : heap block) (rho2 : env) (H2 : heap block)
+             (c : cTag) (Γ : var) (FVs : list var) :
+    (forall j, FV_inv k j GII GI b rho1 H1 rho2 H2 c Γ FVs) ->    
+    image b (reach' H1 (env_locs rho1 (FromList FVs))) <-->
+    (reach' H2 (post H2 (env_locs rho2 ([set Γ])))).
+  Proof.
+    intros Hfv. split.
+    - intros l' [l [[m [Hm Hr]] Heq]].
+      eexists m. split; eauto. eapply FV_inv_image_post. eauto.
+      eexists; split; eauto.
+    - intros l' [m [Hm Hr]].
+      eapply FV_inv_image_post in Hr; eauto.
+      destruct Hr as [l [Heql Hin]]. eexists; split; eauto.
+      eexists; split; eauto.
+  Qed.
+
+  (** * Lemmas about [FV_inv] *)
+  Lemma FV_inv_weak_in_FV_inv k j P1 P2 rho1 H1 rho2 H2 β c Γ FVs :
+    FV_inv k j P1 P2 β rho1 H1 rho2 H2 c Γ FVs ->
+    FV_inv_weak rho1 rho2 H2 c Γ FVs.
+  Proof.
+    intros (x1 & x2 & l & Hget1 & Hget2 & Hall).
+    repeat eexists; eauto.
+    eapply Forall2_monotonic; [| eassumption ].
+    now firstorder.
+  Qed.
+
+  (** * Lemmas about [Fun_inv] *)
+
+  Lemma Fun_inv_image_post (k j : nat) (GII : GIInv) (GI : GInv) (b : Inj)
+             (rho1 : env) (H1 : heap block) (rho2 : env) (H2 : heap block)
+             (Scope Funs : Ensemble var) (σ : var -> var) :
+    Fun_inv k j GII GI b rho1 H1 rho2 H2 Scope Funs σ ->
+    image b ((post H1 ^ j) (env_locs rho1 Funs)) <-->
+          (post H2 ^ j) (env_locs rho2 (image σ Funs)).
+  Proof.
+    intros Hfun. split.
+    - intros l [l' [Hin Heq]]. subst.
+      edestruct post_n_exists_Singleton as [l'' [Hpost' Hin']]; eauto.
+      edestruct Hpost' as [f [Hinf Hgetf]].
+      edestruct Hfun as (lf1 & lf2 & Hget1 & Hget2 & Hrel); eauto. 
+      rewrite Hget1 in Hgetf.
+      eapply cc_approx_val_image_eq in Hrel.
+      eapply post_n_set_monotonic.
+      eapply env_locs_monotonic.
+      eapply Singleton_Included. eexists; split; eauto.
+      eapply post_n_set_monotonic. eapply env_locs_Singleton; eauto.
+      eapply Hrel. eexists; split;  eauto.
+      eapply post_n_set_monotonic; eauto. eapply Singleton_Included. eassumption.
+    - intros l Hpost.
+      edestruct post_n_exists_Singleton as [l'' [Hpost' Hin']]; eauto.
+      edestruct Hpost' as [f' [[f'' [Hinf' Heq]] Hgetf]]; subst.
+      edestruct Hfun as (lf1 & lf2 & Hget1 & Hget2 & Hrel); eauto.
+      eapply cc_approx_val_image_eq in Hrel.
+      rewrite Hget2 in Hgetf. destruct lf2; inv Hgetf. eapply Hrel in Hin'.
+      eapply image_monotonic; eauto.
+      eapply post_n_set_monotonic. eexists; split; eauto.
+      rewrite Hget1; eauto.
+  Qed.
+
+  Lemma Fun_inv_j_monotonic (k j' j : nat) (GII : GIInv) (GI : GInv) (b : Inj)
+        (rho1 : env) (H1 : heap block) (rho2 : env) (H2 : heap block)
+        (Scope Funs : Ensemble var) (σ : var -> var) :
+    Fun_inv k j GII GI b rho1 H1 rho2 H2 Scope Funs σ  ->
+    j' <= j ->
+    Fun_inv k j' GII GI b rho1 H1 rho2 H2 Scope Funs σ .
+  Proof.
+    intros Hfv Hlt f Hin'.
+    edestruct Hfv as (lf1 & lf2 & Hget1 & Hget2 & Hrel); eauto.
+    repeat eexists; eauto.
+    eapply cc_approx_val_j_monotonic; eauto.
+  Qed.
+
+  Lemma Fun_inv_set_not_in_Funs_r (k  j : nat) (GII : GIInv) (GI : GInv) (b : Inj)
+        (rho1 : env) (H1 : heap block) (rho2 : env) (H2 : heap block)
+        (Scope Funs : Ensemble var) (σ : var -> var) x v :
+    Fun_inv k j GII GI b rho1 H1 rho2 H2 Scope Funs σ  ->
+    ~ x \in (image σ Funs) ->
+    Fun_inv k j GII GI b rho1 H1 (M.set x v rho2) H2 Scope Funs σ .
+  Proof.
+    intros Hfv Hlt f Hin'.
+    edestruct Hfv as (lf1 & lf2 & Hget1 & Hget2 & Hrel); eauto.
+    repeat eexists; eauto.
+    rewrite M.gso; eauto. intros Hc; inv Hc; eauto.
+    eapply Hlt; eexists; split; eauto.
+  Qed.
+  
+  Lemma Fun_inv_image_reach (k : nat) (GII : GIInv) (GI : GInv) (b : Inj)
+             (rho1 : env) (H1 : heap block) (rho2 : env) (H2 : heap block)
+             (Scope Funs : Ensemble var) (σ : var -> var) :
+    (forall j, Fun_inv k j GII GI b rho1 H1 rho2 H2 Scope Funs σ) ->
+    image b (reach' H1 (env_locs rho1 Funs)) <-->
+    reach' H2 (env_locs rho2 (image σ Funs)).
+  Proof.
+    intros Hfv. split.
+    - intros l' [l [[m [Hm Hr]] Hin]].
+      eexists m. split; eauto. eapply Fun_inv_image_post. eauto.
+      eexists; split; eauto.
+    - intros l' [m [Hm Hr]].
+      eapply Fun_inv_j_monotonic in Hfv; eauto.
+      eapply Fun_inv_image_post in Hr; eauto.
+      destruct Hr as [l [Heql Hin]]. eexists; split; eauto.
+      eexists; split; eauto.
+  Qed.
+  
+  Lemma Fun_inv_image_reach_n
+        (k j : nat) (GII : GIInv) (GI : GInv) (b : Inj)
+        (rho1 : env) (H1 : heap block) (rho2 : env) (H2 : heap block)
+        (Scope Funs : Ensemble var) (σ : var -> var) :
+    Fun_inv k j GII GI b rho1 H1 rho2 H2 Scope Funs σ ->
+    image b (reach_n H1 j (env_locs rho1 Funs)) <-->
+    (reach_n H2 j) (env_locs rho2 (image σ Funs)).
+  Proof.
+    intros Hfv. split.
+    - intros l' [l [[m [Hm Hr]] Hin]].
+      eapply Fun_inv_j_monotonic in Hfv; eauto.
+      eexists m. split; eauto. eapply Fun_inv_image_post. eassumption.
+      eexists; split; eauto.
+    - intros l' [m [Hm Hr]].
+      eapply Fun_inv_j_monotonic in Hfv; eauto.
+      eapply Fun_inv_image_post in Hr; eauto.
+      destruct Hr as [l [Heql Hin]]. eexists; split; eauto.
+      eexists; split; eauto.
+  Qed.
+
+  Lemma Fun_inv_weak_in_Fun_inv k j P1 P2 rho1 H1 rho2 H2 β Scope Funs σ :
+    Fun_inv k j P1 P2 β rho1 H1 rho2 H2 Scope Funs σ  ->
+    Fun_inv_weak rho1 H1 rho2 H2 Scope Funs σ.
+  Proof.
+    now firstorder. 
+  Qed.
+
+
   (** * Postcondition *)
   (** Enforces that the resource consumption of the target is within certain bounds *)
   Definition Post
@@ -128,8 +305,8 @@ Module ClosureConversionCorrect (H : Heap).
   Proof.
     simpl. intros H. omega.
   Qed.
-
-
+  
+  
   (** TODO move *)
 
   Lemma ctx_to_heap_env_size_heap C rho1 rho2 H1 H2 c :
@@ -173,17 +350,14 @@ Module ClosureConversionCorrect (H : Heap).
   (** * Lemmas about [project_var] and [project_vars] *)
   
   Lemma project_var_get Scope Funs σ c Γ FVs S1 x x' C1 S2 rho1 H1 rho2 H2 m y:
-    project_var clo_tag Scope Funs σ c Γ FVs S1 x x' C1 S2 ->
+    project_var Scope Funs σ c Γ FVs S1 x x' C1 S2 ->
     ctx_to_heap_env C1 H1 rho1 H2 rho2 m ->
     ~ In _ S1 y ->
     M.get y rho1 = M.get y rho2. 
   Proof.
     intros Hvar Hctx Hin. inv Hvar.
     - inv Hctx. reflexivity.
-    - inv Hctx.
-      destruct (var_dec y x'); subst.
-      contradiction.
-      inv H16. now rewrite M.gso.
+    - inv Hctx. reflexivity.
     - inv Hctx. inv H19.
       destruct (var_dec y x'); subst.
       contradiction.
@@ -191,7 +365,7 @@ Module ClosureConversionCorrect (H : Heap).
   Qed.    
   
   Lemma project_vars_get Scope Funs σ c Γ FVs S1 xs xs' C1 S2 rho1 H1 rho2 H2 m y:
-    project_vars clo_tag Scope Funs σ c Γ FVs S1 xs xs' C1 S2 ->
+    project_vars Scope Funs σ c Γ FVs S1 xs xs' C1 S2 ->
     ctx_to_heap_env C1 H1 rho1 H2 rho2 m ->
     ~ In _ S1 y ->
     M.get y rho1 = M.get y rho2. 
@@ -209,7 +383,7 @@ Module ClosureConversionCorrect (H : Heap).
   Qed.
   
   Lemma project_var_getlist Scope Funs σ c Γ FVs S1 x x' C1 S2 rho1 H1 rho2 H2 m ys :
-    project_var clo_tag Scope Funs σ c Γ FVs S1 x x' C1 S2 ->
+    project_var Scope Funs σ c Γ FVs S1 x x' C1 S2 ->
     ctx_to_heap_env C1 H1 rho1 H2 rho2 m ->
     Disjoint _ S1 (FromList ys) ->
     getlist ys rho1 = getlist ys rho2. 
@@ -226,7 +400,7 @@ Module ClosureConversionCorrect (H : Heap).
 
 
   Lemma project_vars_getlist Scope Funs σ c Γ FVs S1 xs xs' C1 S2 rho1 H1 rho2 H2 m ys :
-    project_vars clo_tag Scope Funs σ c Γ FVs S1 xs xs' C1 S2 ->
+    project_vars Scope Funs σ c Γ FVs S1 xs xs' C1 S2 ->
     ctx_to_heap_env C1 H1 rho1 H2 rho2 m ->
     Disjoint _ S1 (FromList ys) ->
     getlist ys rho1 = getlist ys rho2. 
@@ -241,37 +415,35 @@ Module ClosureConversionCorrect (H : Heap).
       intros Hc. eapply Hnin. eauto.
   Qed.        
   
-  Lemma project_var_ctx_to_heap_env Scope Funs σ c Γ FVs x x' C S S' v1 rho1 rho2 H2:
-    project_var clo_tag Scope Funs σ c Γ FVs S x x' C S' ->
-    Fun_inv_weak rho1 rho2 Scope Funs σ c Γ ->
-    FV_inv_weak rho1 rho2 H2 Scope Funs c Γ FVs ->
+  Lemma project_var_ctx_to_heap_env Scope Funs σ c Γ FVs x x' C S S' v1 rho1 rho2 H1 H2:
+    project_var Scope Funs σ c Γ FVs S x x' C S' ->
+    Fun_inv_weak rho1 H1 rho2 H2 Scope Funs σ  ->
+    FV_inv_weak rho1 rho2 H2 c Γ FVs ->
     M.get x rho1 = Some v1 ->
     exists H2' rho2' s, ctx_to_heap_env C H2 rho2 H2' rho2' s.
   Proof.
     intros Hproj HFun HFV Hget. inv Hproj.
     - repeat eexists; econstructor; eauto.
     - edestruct HFun as
-          [vf [venv [Hnin [Hget1 Hget2]]]]; eauto.
-      destruct (alloc (Constr clo_tag [vf; venv]) H2) as [l' H2'] eqn:Hal.
-      repeat eexists; econstructor; eauto.
-      simpl. rewrite Hget2, Hget1. reflexivity. constructor.
-    - edestruct HFV as [v [vs [l [v' [Hgetv [Hget1 [Hget2 Hnth']]]]]]]; eauto.
+          (vf1 & vf4 & Hget1 & Hget2) ; eauto.
+      repeat eexists; constructor; eauto.
+    - edestruct HFV as (v & vs & l & Hget1 & Hget2 & Hall).
+      edestruct (Forall2_nthN _ FVs vs N x Hall) as [v' [Hnth [v'' Hget'']]]; eauto.
       repeat eexists. econstructor; eauto. constructor. 
   Qed.
   
-  Lemma project_vars_ctx_to_heap_env Scope Funs σ c Γ FVs xs xs' C S S' vs1 rho1 rho2 H2:
+  Lemma project_vars_ctx_to_heap_env Scope Funs σ c Γ FVs xs xs' C S S' vs1 rho1 H1 rho2 H2:
     Disjoint _ S (Union var Scope
-                        (Union var (image σ (Setminus _ Funs Scope))
+                        (Union var (image σ Funs)
                                (Union var (FromList FVs) (Singleton var Γ)))) ->
     
-    project_vars clo_tag Scope Funs σ c Γ FVs S xs xs' C S' ->
-    Fun_inv_weak rho1 rho2 Scope Funs σ c Γ ->
-    FV_inv_weak rho1 rho2 H2 Scope Funs c Γ FVs ->
+    project_vars Scope Funs σ c Γ FVs S xs xs' C S' ->
+    Fun_inv_weak rho1 H1 rho2 H2 Scope Funs σ ->
+    FV_inv_weak rho1 rho2 H2 c Γ FVs ->
     getlist xs rho1 = Some vs1 ->
     exists H2' rho2' s, ctx_to_heap_env C H2 rho2 H2' rho2' s.
   Proof.
     intros HD Hvars HFun HFV.
-    (* assert (HD' := Hvars). *)
     revert Scope Funs Γ FVs xs' C S S' vs1
            rho1 rho2 H2 HD  Hvars HFun HFV.
     induction xs;
@@ -279,25 +451,20 @@ Module ClosureConversionCorrect (H : Heap).
              rho1 rho2 H2 HD Hvars HFun HFV Hgetlist.
     - inv Hvars. repeat eexists; econstructor; eauto.
     - inv Hvars. simpl in Hgetlist.
-      destruct (M.get a rho1) eqn:Hgeta1; try discriminate. 
+      destruct (M.get a rho1) eqn:Hgeta1; try discriminate.
       destruct (getlist xs rho1) eqn:Hgetlist1; try discriminate.
       edestruct project_var_ctx_to_heap_env with (rho1 := rho1) as [H2' [rho2' [s Hctx1]]]; eauto.
       inv Hgetlist.
       edestruct IHxs with (H2 := H2') (rho2 := rho2') as [H2'' [rho2'' [s' Hctx2]]]; [| eassumption | | | eassumption | ].
       + eapply Disjoint_Included_l; [| eassumption ].
         eapply project_var_free_set_Included. eassumption.
-      + intros f v' Hnin Hin Hget.
-        edestruct HFun as
-            [vf [venv [Hnin' [Hget1 Hget2]]]]; eauto.
+      + intros f Hin.
+        edestruct HFun as (vf1 & vf2 & Hgetf1 & Hgetf2); try eassumption.
         repeat eexists; eauto.
-        * erewrite <- project_var_get; try eassumption.
-          intros Hin'. eapply HD. constructor. now eauto.
-          right. left. eexists. now eauto.
-        * erewrite <- project_var_get; try eassumption.
-          intros Hin'. eapply HD. constructor. now eauto.
-          right. right. right. reflexivity.
-      + intros x N Hnin1 Hnin2 Hnth.
-        edestruct HFV as [v' [vs [l' [v'' [Hget [Hget1 [Hget2 Hnth']]]]]]]; eauto.
+        erewrite <- project_var_get; try eassumption.
+        intros Hin'. eapply HD. constructor. now eauto.
+        right. left. eexists. split; eauto.
+      + edestruct HFV as [v' [vs [l' [Hget [Hget1 Hall]]]]]; eauto.
         repeat eexists; eauto.
         * erewrite <- project_var_get; try eassumption.
           intros Hin'. eapply HD. constructor. now eauto.
@@ -309,19 +476,15 @@ Module ClosureConversionCorrect (H : Heap).
 
   (** [project_var] preserves env_locs in dom *)
   Lemma project_var_env_locs Scope Funs σ c Γ FVs x x' C S S' e k rho H rho' H':
-    project_var clo_tag Scope Funs σ c Γ FVs S x x' C S' ->
+    project_var Scope Funs σ c Γ FVs S x x' C S' ->
     ctx_to_heap_env C H rho H' rho' k ->
     well_formed (reach' H (env_locs rho (occurs_free (C |[ e ]|)))) H ->
     env_locs rho (occurs_free (C |[ e ]|)) \subset dom H ->
     env_locs rho' (occurs_free e) \subset dom  H'.
   Proof with (now eauto with Ensembles_DB). 
     intros Hvar Hctx Hlocs Hwf. inv Hvar; inv Hctx.
-    - simpl; eauto.
-    - inv H15.
-      rewrite HL.alloc_dom; [| eassumption ].
-      eapply Included_trans. eapply env_locs_set_Inlcuded'.
-      eapply Included_Union_compat. reflexivity.
-      eapply Included_trans; [| eassumption ]. simpl. normalize_occurs_free...
+    - simpl in *; eauto.
+    - simpl in *; eauto.
     - inv H18.
       eapply Included_trans. eapply env_locs_set_Inlcuded'.
       simpl. eapply Union_Included.
@@ -336,10 +499,40 @@ Module ClosureConversionCorrect (H : Heap).
         eapply nthN_In. eassumption.
       + eapply Included_trans; [| eassumption ]. simpl. normalize_occurs_free...
   Qed.
+  
+  Lemma project_var_env_locs' Scope Funs σ c Γ FVs x x' C S S' k rho H rho' H':
+    project_var Scope Funs σ c Γ FVs S x x' C S' ->
+    ctx_to_heap_env C H rho H' rho' k ->
+    well_formed (reach' H (env_locs rho (Scope :|: (image σ Funs) :|: [set Γ]))) H ->
+    env_locs rho (Scope :|: (image σ Funs) :|: [set Γ]) \subset dom H ->
+    env_locs rho' (x' |: Scope :|: (image σ Funs) :|: [set Γ]) \subset dom  H'.
+  Proof with (now eauto with Ensembles_DB). 
+    intros Hvar Hctx Hlocs Hwf. inv Hvar; inv Hctx.
+    - rewrite (Union_Same_set [set x']). eassumption.
+      eapply Singleton_Included; eauto.
+    - rewrite (Union_commut [set (σ x)]).
+      rewrite <- (Union_assoc Scope). rewrite (Union_Same_set [set _]). eassumption.
+      eapply Singleton_Included; eauto. eexists; split; eauto.
+    - inv H18.
+      eapply Included_trans. eapply env_locs_set_Inlcuded'.
+      simpl. eapply Union_Included.
+      + eapply Included_trans; [| eapply reachable_in_dom; eauto ].
+        rewrite !env_locs_Union, !reach'_Union.
+        eapply Included_Union_preserv_r. 
+        erewrite (reach_unfold H' (env_locs rho ([set _ ]))).
+        eapply Included_Union_preserv_r. 
+        eapply Included_trans; [| eapply reach'_extensive ].
+        rewrite env_locs_Singleton; eauto.
+        simpl. rewrite post_Singleton; eauto.
+        simpl. eapply In_Union_list. eapply in_map.
+        eapply nthN_In. eassumption.
+      + eapply Included_trans; [| eassumption ]. simpl.
+        eapply env_locs_monotonic. now eauto 20 with Ensembles_DB.
+  Qed.
 
   (** [project_var] preserves well-formedness *)
   Lemma project_var_well_formed Scope Funs σ c Γ FVs x x' C S S' e k rho H rho' H':
-    project_var clo_tag Scope Funs σ c Γ FVs S x x' C S' ->
+    project_var Scope Funs σ c Γ FVs S x x' C S' ->
     ctx_to_heap_env C H rho H' rho' k ->
     (env_locs rho (occurs_free (C |[ e ]|))) \subset dom H ->
     well_formed (reach' H (env_locs rho (occurs_free (C |[ e ]|)))) H ->
@@ -347,20 +540,7 @@ Module ClosureConversionCorrect (H : Heap).
   Proof with (now eauto with Ensembles_DB). 
     intros Hvar Hctx Hlocs Hwf. inv Hvar; inv Hctx.
     - simpl; eauto.
-    - inv H15.
-      eapply well_formed_antimon; [| eapply well_formed_reach_alloc; try eassumption ].
-      + eapply reach'_set_monotonic. eapply env_locs_monotonic.
-        simpl. normalize_occurs_free.
-        rewrite <- Union_assoc.
-        eapply Included_Union_preserv_r. eapply Included_Union_Setminus.
-        now eauto with typeclass_instances.
-      + simpl. normalize_occurs_free. rewrite env_locs_Union, reach'_Union; eauto.
-        eapply Included_Union_preserv_l.
-        rewrite !FromList_cons, !FromList_nil, !env_locs_Union, env_locs_Empty_set, Union_Empty_set_neut_r.
-        simpl in *. destruct (M.get (σ x) rho) eqn:Hget; try congruence.
-        destruct (M.get Γ rho) eqn:Hget'; try congruence. inv H13.
-        simpl. rewrite Union_Empty_set_neut_r. rewrite !env_locs_Singleton; try eassumption.
-        eapply reach'_extensive.
+    - simpl; eauto.
     - inv H18.
       eapply well_formed_antimon; [| eapply well_formed_reach_set; try eassumption ].
       + eapply reach'_set_monotonic. eapply env_locs_monotonic.
@@ -378,12 +558,106 @@ Module ClosureConversionCorrect (H : Heap).
         eapply nthN_In. eassumption.
   Qed.
 
-  Lemma project_vars_env_locs Scope Funs σ c Γ FVs xs xs' C S S' e k rho H rho' H':
-    project_vars clo_tag Scope Funs σ c Γ FVs S xs xs' C S' ->
+  (** [project_var] preserves well-formedness *)
+  Lemma project_var_well_formed' Scope Funs σ c Γ FVs x x' C S S' k rho H rho' H':
+    project_var Scope Funs σ c Γ FVs S x x' C S' ->
     ctx_to_heap_env C H rho H' rho' k ->
+    (env_locs rho (Scope :|: (image σ Funs) :|: [set Γ])) \subset dom H ->
+    well_formed (reach' H (env_locs rho (Scope :|: (image σ Funs) :|: [set Γ]))) H ->
+    well_formed (reach' H' (env_locs rho' (x' |: Scope :|: (image σ Funs) :|: [set Γ]))) H'.
+  Proof with (now eauto with Ensembles_DB). 
+    intros Hvar Hctx Hlocs Hwf. inv Hvar; inv Hctx.
+    - simpl; eauto. rewrite (Union_Same_set [set x']). eassumption.
+      eapply Singleton_Included...
+    - rewrite (Union_commut [set (σ x)]).
+      rewrite <- (Union_assoc Scope). rewrite (Union_Same_set [set _]). eassumption.
+      eapply Singleton_Included; eauto. eexists; split; eauto.
+    - inv H18.
+      eapply well_formed_antimon; [| eapply well_formed_reach_set; try eassumption ].
+      + eapply reach'_set_monotonic. eapply env_locs_monotonic.
+        now eauto 20 with Ensembles_DB.
+      + simpl. eapply well_formed_antimon; try eassumption.
+        rewrite !env_locs_Union, !reach'_Union.
+        eapply Included_Union_preserv_r. 
+        erewrite (reach_unfold H' (env_locs rho ([set _ ]))).
+        eapply Included_Union_preserv_r. 
+        eapply reach'_set_monotonic.
+        rewrite env_locs_Singleton; eauto.
+        simpl. rewrite post_Singleton; eauto.
+        simpl. eapply In_Union_list. eapply in_map.
+        eapply nthN_In. eassumption.
+  Qed.
+
+  Lemma project_var_env_locs_subset Scope Funs σ c Γ FVs xs xs' C S S' S1 k rho H rho' H':
+    project_var Scope Funs σ c Γ FVs S xs xs' C S' ->
+    ctx_to_heap_env C H rho H' rho' k ->
+    Disjoint _ S1 S ->
+    env_locs rho' S1 \subset env_locs rho S1.
+  Proof with (now eauto with Ensembles_DB). 
+    intros Hvar Hctx HD. destruct Hvar; inv Hctx; try reflexivity.
+    - inv H18. rewrite env_locs_set_not_In.
+      eapply env_locs_monotonic...
+      intros Hc; eapply HD; eauto.
+  Qed.
+
+   Lemma project_vars_env_locs_subset Scope Funs σ c Γ FVs xs xs' C S S' S1 k rho H rho' H':
+    project_vars Scope Funs σ c Γ FVs S xs xs' C S' ->
+    ctx_to_heap_env C H rho H' rho' k ->
+    Disjoint _ S1 S ->
+    env_locs rho' S1 \subset env_locs rho S1.
+  Proof with (now eauto with Ensembles_DB). 
+    intros Hvar. revert rho H rho' H' k. 
+    induction Hvar; intros rho1 H1 rho2 H2 k Hctx Hd.
+    - inv Hctx. reflexivity.
+    - edestruct ctx_to_heap_env_comp_ctx_f_l as [rho3 [H3 [m1 [m2 [Hctx2 [Hctx3 Heq]]]]]].
+      eassumption. subst.
+      eapply Included_trans. eapply IHHvar; eauto.
+      eapply Disjoint_Included_r; try eassumption.
+      eapply project_var_free_set_Included; eauto.
+      eapply project_var_env_locs_subset; eauto.
+  Qed.
+
+  Lemma project_var_not_In_free_set' Scope Funs σ c Γ FVs x x' C S S'  :
+    project_var Scope Funs σ c Γ FVs S x x' C S' ->
+    Disjoint _ S (Scope :|: (image σ Funs)) ->
+    ~ In _ S' x'.
+  Proof.
+    intros Hproj Hd. inv Hproj; intros Hc.
+    - eapply Hd. eauto.
+    - eapply Hd; eauto. constructor; eauto. right.
+      eexists; eauto.
+    - inv Hc. exfalso. eauto.    
+  Qed.
+
+  Lemma project_var_heap Scope Funs σ c Γ FVs x x' S S' C H rho H' rho' k :
+    project_var Scope Funs σ c Γ FVs S x x' C S' ->
+    ctx_to_heap_env C H rho H' rho' k ->
+    H = H'. 
+  Proof.
+    intros Hvar Hctx; inv Hvar; inv Hctx; eauto.
+    inv H18; eauto.
+  Qed.
+
+  Lemma project_vars_heap Scope Funs σ c Γ FVs x x' S S' C H rho H' rho' k :
+    project_vars Scope Funs σ c Γ FVs S x x' C S' ->
+    ctx_to_heap_env C H rho H' rho' k ->
+    H = H'. 
+  Proof.
+    intros Hvar. revert rho H rho' H' k. 
+    induction Hvar; intros rho1 H1 rho2 H2 k Hctx.
+    - inv Hctx; eauto.
+    - edestruct ctx_to_heap_env_comp_ctx_f_l as [rho3 [H3 [m1 [m2 [Hctx2 [Hctx3 Heq]]]]]].
+      eassumption. subst.
+      eapply project_var_heap in Hctx2; eauto.
+      subst. eapply IHHvar; eauto.
+  Qed.
+
+  Lemma project_vars_env_locs Scope Funs σ c Γ FVs xs xs' C S S' e k rho H rho' H':
+    project_vars Scope Funs σ c Γ FVs S xs xs' C S' ->
+    ctx_to_heap_env C H rho H' rho' k ->
+    (env_locs rho (occurs_free (C |[ e ]|))) \subset dom H ->
     well_formed (reach' H (env_locs rho (occurs_free (C |[ e ]|)))) H ->
-    env_locs rho (occurs_free (C |[ e ]|)) \subset dom H ->
-    env_locs rho' (occurs_free e) \subset dom  H'.
+    (env_locs rho' (occurs_free e)) \subset dom H'.
   Proof with (now eauto with Ensembles_DB). 
     intros Hvar. revert rho H rho' H' k e. 
     induction Hvar; intros rho1 H1 rho2 H2 k e Hctx Hlocs Hwf.
@@ -392,13 +666,45 @@ Module ClosureConversionCorrect (H : Heap).
       eassumption. subst.
       rewrite <- app_ctx_f_fuse in *.
       eapply IHHvar; try eassumption.
-      eapply project_var_well_formed; try eassumption.
-      eapply project_var_env_locs; try eassumption. 
+      eapply project_var_env_locs; try eassumption.
+      eapply project_var_well_formed; try eassumption. 
+  Qed.
+    
+  Lemma project_vars_env_locs' Scope Funs σ c Γ FVs xs xs' C S S' k rho H rho' H':
+    project_vars Scope Funs σ c Γ FVs S xs xs' C S' ->
+    ctx_to_heap_env C H rho H' rho' k ->
+    Disjoint _ S (Scope :|: (image σ Funs)) ->
+    well_formed (reach' H (env_locs rho (Scope :|: (image σ Funs) :|: [set Γ]))) H ->
+    env_locs rho (Scope :|: (image σ Funs) :|: [set Γ]) \subset dom H ->
+    env_locs rho' (FromList xs' :|: Scope :|: (image σ Funs) :|: [set Γ]) \subset dom  H'.
+  Proof with (now eauto with Ensembles_DB). 
+    intros Hvar. revert rho H rho' H' k. 
+    induction Hvar; intros rho1 H1 rho2 H2 k Hctx Hd Hlocs Hwf.
+    - inv Hctx. rewrite FromList_nil, Union_Empty_set_neut_l. simpl in *; eauto.
+    - edestruct ctx_to_heap_env_comp_ctx_f_l as [rho3 [H3 [m1 [m2 [Hctx2 [Hctx3 Heq]]]]]].
+      eassumption. subst.
+      rewrite FromList_cons.
+      rewrite <- !Union_assoc. rewrite env_locs_Union.
+      eapply Union_Included.
+      eapply Included_trans.
+      eapply project_vars_env_locs_subset. eassumption. eassumption.
+      eapply Disjoint_Singleton_l. eapply project_var_not_In_free_set'. eassumption.
+      eapply Disjoint_Included_r; [| eassumption ]...
+      erewrite <- project_vars_heap with (H := H3) (H' := H2); eauto .
+      eapply Included_trans; [| eapply project_var_env_locs'; eauto ].
+      eapply env_locs_monotonic...
+      rewrite !Union_assoc.
+      eapply IHHvar; eauto.
+      eapply Disjoint_Included_l. eapply project_var_free_set_Included. eassumption.
+      eassumption.
+      eapply well_formed_antimon; [| eapply project_var_well_formed'; eauto ].
+      eapply reach'_set_monotonic. eapply env_locs_monotonic...
+      eapply Included_trans; [| eapply project_var_env_locs'; eauto ].
+      eapply env_locs_monotonic...
   Qed.
   
-  
   Lemma project_vars_well_formed Scope Funs σ c Γ FVs xs xs' C S S' e k rho H rho' H':
-    project_vars clo_tag Scope Funs σ c Γ FVs S xs xs' C S' ->
+    project_vars Scope Funs σ c Γ FVs S xs xs' C S' ->
     ctx_to_heap_env C H rho H' rho' k ->
     (env_locs rho (occurs_free (C |[ e ]|))) \subset dom H ->
     well_formed (reach' H (env_locs rho (occurs_free (C |[ e ]|)))) H ->
@@ -414,122 +720,337 @@ Module ClosureConversionCorrect (H : Heap).
       eapply project_var_env_locs; try eassumption.
       eapply project_var_well_formed; try eassumption. 
   Qed.
-
-  Require Import tactics.
-
-  (** Correctness of [project_var] *)
-  Lemma project_var_correct GII GI k j H1 rho1 H2 rho2 H2' rho2' b
-        Scope Funs σ c Γ FVs x x' C S S' m :
-    project_var clo_tag Scope Funs σ c Γ FVs S x x' C S' ->
-    
-    (H1, rho1) ⋞ ^ (Scope; k; j; GII; GI; b) (H2, rho2) ->
-    Fun_inv k GII GI b rho1 H1 rho2 H2 Scope Funs σ c Γ ->
-    FV_inv k GII GI b rho1 H1 rho2 H2 Scope Funs c Γ FVs ->
-    ctx_to_heap_env C H2 rho2 H2' rho2' m ->
-    injective_subdomain (reach' H1 (env_locs rho1 (Scope :|: Funs))) b ->
-    
-    Disjoint _ S (Union var Scope
-                        (Union var (image σ (Setminus _ Funs Scope))
-                               (Union var (FromList FVs) (Singleton var Γ)))) ->
-
-    ~ In _ S' x' /\
-    exists b',
-      injective_subdomain (reach' H1 (env_locs rho1 (Scope :|: Funs :|: [set x]))) b' /\
-      (H1, rho1) ⋞ ^ (Scope; k; j; GII; GI; b') (H2', rho2')  /\
-      Fun_inv k GII GI b' rho1 H1 rho2' H2' Scope Funs σ c Γ /\
-      FV_inv k GII GI b' rho1 H1 rho2' H2' Scope Funs c Γ FVs /\
-      cc_approx_var_env k j GII GI b' H1 rho1 H2' rho2' x x'.
-  Proof with (now eauto with Ensembles_DB).
-    intros Hproj Hcc Hfun Henv Hctx Hinj Hd.
-    inv Hproj.
-    - inv Hctx. split. intros Hc. eapply Hd; eauto.
-      eexists. repeat split; eauto. 
-      eapply injective_subdomain_antimon. eassumption.
+  
+  Lemma project_vars_well_formed' Scope Funs σ c Γ FVs xs xs' C S S' k rho H rho' H':
+    project_vars Scope Funs σ c Γ FVs S xs xs' C S' ->
+    ctx_to_heap_env C H rho H' rho' k ->
+    Disjoint _ S (Scope :|: (image σ Funs)) ->
+    (env_locs rho (Scope :|: (image σ Funs) :|: [set Γ])) \subset dom H ->
+    well_formed (reach' H (env_locs rho (Scope :|: (image σ Funs) :|: [set Γ]))) H ->
+    well_formed (reach' H' (env_locs rho' (FromList xs' :|: Scope :|: (image σ Funs) :|: [set Γ]))) H'.
+  Proof with (now eauto with Ensembles_DB). 
+    intros Hvar. revert rho H rho' H' k. 
+    induction Hvar; intros rho1 H1 rho2 H2 k Hctx HD Hlocs Hwf.
+    - inv Hctx. simpl in *; eauto.
+      rewrite FromList_nil, Union_Empty_set_neut_l. simpl in *; eauto.
+    - edestruct ctx_to_heap_env_comp_ctx_f_l as [rho3 [H3 [m1 [m2 [Hctx2 [Hctx3 Heq]]]]]].
+      eassumption. subst.
+      rewrite FromList_cons.
+      rewrite <- !Union_assoc. rewrite env_locs_Union, reach'_Union.
+      eapply well_formed_Union.
+      erewrite <- project_vars_heap with (H := H3) (H' := H2); eauto .
+      eapply well_formed_antimon. eapply reach'_set_monotonic.
+      eapply project_vars_env_locs_subset. eassumption. eassumption.
+      eapply Disjoint_Singleton_l. eapply project_var_not_In_free_set'. eassumption.
+      eapply Disjoint_Included_r; [| eassumption ]...
+      eapply well_formed_antimon; [| eapply project_var_well_formed' ]; eauto.
       eapply reach'_set_monotonic. eapply env_locs_monotonic...
-    - inv Hctx. inv H16.
-      edestruct Hfun as [lf1 [f1 [env1 [Hgetx [Hnin1 [Hnin2 [Hget1 [Hget2 Hclo]]]]]]]]; eauto.
-      simpl in H14. rewrite Hget1, Hget2 in H14. inv H14. split; [| exists (b {lf1 ~> l}); repeat split ].
-      + intros Hc. inv Hc. eauto.
-      + eapply injective_subdomain_extend'. 
-        eapply injective_subdomain_antimon. eassumption.
-        rewrite <- Union_assoc, (Union_commut _ [set x]).
-        rewrite (Union_Same_set [set x])...
-        admit. 
-      + (* not in Scope r + extend *)
-        admit.
-      + intros f Hnin Hin.
-        edestruct Hfun as [lf1' [f1' [env1' [Hgetx' [Hnin1' [Hnin2' [Hget1' [Hget2' Hclo']]]]]]]]; eauto.
-        repeat subst_exp. 
-        do 3 eexists. repeat split; eauto.
-
-        rewrite M.gso; eauto.  intros Heq; subst. eapply Hd.
-        split; eauto. right. left. eexists; split; eauto. now constructor; eauto.
-
-        rewrite M.gso; eauto. intros Heq; subst. now eapply Hd; eauto.
-        
-        intros l_clo1 vs1 Hget j'. repeat subst_exp.
-        srewrite env_locs_Union. eapply reach'_set_monotonic.
-        e
-                                             eapply cc_approx_env_P_set_not_in_P_r. eassumption.
-        intros Hc. eapply Hd. eauto.
-      + (* TODO : make lemma *)
-        intros f v Hnin Hin Hget.
-        edestruct Hfun as
-            [vs [rho3 [B3 [f3 [rho4 [B4 [f4 [Hget1 [Heq2 [Ηnin2 [Hget2 Happrox]]]]]]]]]]]; eauto.
-        subst. repeat eexists; eauto.
-        rewrite M.gso; [ eassumption | now intros Heq; subst; eapply Hd; eauto ].
-        rewrite M.gso. eassumption. 
-        intros Hc. subst; eapply Hd; constructor; eauto. right; left.
-        eexists. split; [| now eauto ]. constructor; eauto.
-      + eapply FV_inv_set_r. now intros Heq; subst; eapply Hd; eauto.
-        eassumption.
-      + intros v Hget. eexists. rewrite M.gss. split; eauto.
-        edestruct Hfun as
-            [vs [rho3 [B3 [f3 [rho4 [B4 [f4 [Hget1 [Heq2 [Ηnin2 [Hget2 Happrox]]]]]]]]]]]; eauto.
-        rewrite Hget2 in H10; inv H10.
-        rewrite Hget1 in H9; inv H9. eassumption.
-    - inv Hctx. inv H12.
-      repeat split; eauto.
-      + intros Hc. inv Hc. eauto.
-      + eapply cc_approx_env_P_set_not_in_P_r. eassumption.
-        intros Hc. eapply Hd. eauto.
-      + intros f' v' Hnin Hin Hget.
-        edestruct Hfun as
-            [vs' [rho3 [B3 [f3 [rho4 [B4 [f4 [Hget1 [Heq2 [Ηnin2 [Hget2 Happrox]]]]]]]]]]]; eauto.
-        subst. repeat eexists; eauto.
-        rewrite M.gso; [ eassumption | now intros Heq; subst; eapply Hd; eauto ].
-        rewrite M.gso. eassumption. 
-        intros Hc. subst; eapply Hd; constructor; eauto. right; left.
-        eexists. split; [| now eauto ]. constructor; eauto.
-      + eapply FV_inv_set_r. now intros Heq; subst; eapply Hd; eauto.
-        eassumption.
-      + intros v' Hget. eexists. rewrite M.gss. split; eauto.
-        edestruct Henv as [vs' [v'' [Hget' [Hnth Hcc']]]]; eauto.
-        rewrite Hget' in H10; inv H10.
-        rewrite H11 in Hnth. now inv Hnth.
+      rewrite !Union_assoc. eapply IHHvar; try eassumption.
+      eapply Disjoint_Included_l. eapply project_var_free_set_Included. eassumption.
+      eassumption.
+      eapply Included_trans; [| eapply project_var_env_locs'; eauto ].
+      eapply env_locs_monotonic...
+      eapply well_formed_antimon; [| eapply project_var_well_formed'; eauto ].
+      eapply reach'_set_monotonic. eapply env_locs_monotonic...
   Qed.
 
-      
-  (** * Lemmas about [Fun_inv] *)
-  Lemma Fun_inv_weak_in_Fun_inv k P1 P2 rho1 H1 rho2 H2 β Scope Funs σ c Γ :
-    Fun_inv k P1 P2 β rho1 H1 rho2 H2 Scope Funs σ c Γ ->
-    Fun_inv_weak rho1 rho2 Scope Funs σ c Γ.
-  Proof.
-    intros HFun f v' Hnin Hin Hget.
-    edestruct HFun as
-        [vf [venv [Hnin' [Hget1 [Hget2 _]]]]]; eauto.
-  Qed.
+  (** TODO move *)
 
-  (** * Lemmas about [FV_inv] *)
-  Lemma FV_inv_weak_in_FV_inv k P1 P2 rho1 H1 rho2 H2 β Scope Funs c Γ FVs :
-    FV_inv k P1 P2 β rho1 H1 rho2 H2 Scope Funs c Γ FVs ->
-    FV_inv_weak rho1 rho2 H2 Scope Funs c Γ FVs.
+  Lemma cc_approx_val_image_reach_eq GIP GP (k : nat) (β : Inj)  (H1 H2 : heap block)
+        (v1 v2 : value) :
+    (forall j, (Res (v1, H1)) ≺ ^ (k ; j ; GIP ; GP ; β) (Res (v2, H2))) ->
+    image β (reach' H1 (val_loc v1)) <--> (reach' H2 (val_loc v2)).
   Proof.
-    intros HFV x N v' Hnin1 Hnin2 Hnth Hget.
-    edestruct HFV as [vs [l' [v'' [Hget1 [Hget2 [Hnth' _]]]]]]; eauto.
-    firstorder.
+    intros Hres. split.
+    - intros l' [l [[m [Hm Hr]] Hin]].
+      eapply cc_approx_val_image_eq in Hres. eexists m.
+      split; eauto. eapply Hres. eexists. split; eauto.
+    - intros l' [m [Hm Hr]].
+      eapply cc_approx_val_image_eq in Hres. eapply Hres in Hr.
+      destruct Hr as [l [Heql Hin]]. eexists; split; eauto.
+      eexists; split; eauto.
   Qed.
   
+  Lemma cc_approx_env_image_reach_eq GIP GP
+        (k : nat) (β : Inj)
+        (H1 H2 : heap block) (rho1 rho2 : env) (x y : var) (v : value) :
+    (forall j, cc_approx_var_env k j GIP GP β H1 rho1 H2 rho2 x y) ->
+    M.get x rho1 = Some v -> 
+    image β (reach' H1 (env_locs rho1 [set x])) <-->
+    reach' H2 (env_locs rho2 [set y]).
+  Proof.
+    intros Hcc Hget.
+    edestruct (Hcc 0) as [v' [Hget' Hv]]; eauto.
+    rewrite !env_locs_Singleton; eauto. 
+    rewrite cc_approx_val_image_reach_eq. reflexivity.
+    intros j; eauto.
+    edestruct (Hcc j) as [v'' [Hget'' Hv']]; eauto.
+    repeat subst_exp. eassumption.
+  Qed.
+
+  Lemma cc_approx_env_image_eq GIP GP S (k j : nat) (β : Inj)
+        (H1 H2 : heap block) (rho1 rho2 : env) :
+    (H1, rho1) ⋞ ^ (S; k; j; GIP; GP; β) (H2, rho2) ->
+    binding_in_map S rho1 ->
+    image β ((post H1 ^ j) (env_locs rho1 S)) <--> (post H2 ^ j) (env_locs rho2 S).
+  Proof.
+    intros Henv Hbin. split.
+    - intros l1 [l2 [Hin Hbeq]].
+      edestruct post_n_exists_Singleton as [l' [Henv' Hp]]. eassumption.
+      destruct Henv' as [x [Hgetx Hinx]].
+      destruct (M.get x rho1) eqn:Hget1; try now inv Hinx.
+      destruct v; inv Hinx; try contradiction.
+      assert (Hget2 := Hget1).
+      eapply cc_approx_var_env_image_eq in Hget1; eauto.
+      eapply post_n_set_monotonic; [| eapply Hget1 ].
+      eapply env_locs_monotonic. now eapply Singleton_Included; eauto.
+      eexists; split; eauto.
+      eapply proper_post_n. eapply env_locs_Singleton. now eauto.
+      eassumption. 
+    - intros l Hp.
+      edestruct post_n_exists_Singleton as [l' [Henv' Hp']]. eassumption.
+      destruct Henv' as [x [Hgetx Hinx]].
+      destruct (M.get x rho2) eqn:Hget1; try now inv Hinx.
+      destruct v; inv Hinx; try contradiction.
+      eapply image_monotonic. eapply post_n_set_monotonic.
+      eapply env_locs_monotonic. eapply Singleton_Included. eassumption.
+      edestruct Hbin as [v Hget]; eauto.
+      edestruct Henv as [l'' [Hget' Hres]]; eauto. 
+      eapply cc_approx_var_env_image_eq; eauto.
+      eapply proper_post_n. now eapply env_locs_Singleton; eauto.
+      subst_exp. eassumption.
+  Qed.
+
+  Lemma cc_approx_env_image_reach_n GIP GP S (k j : nat) (β : Inj)
+        (H1 H2 : heap block) (rho1 rho2 : env) :
+    (H1, rho1) ⋞ ^ (S; k; j; GIP; GP; β) (H2, rho2) ->
+    binding_in_map S rho1 ->
+    image β ((reach_n H1 j) (env_locs rho1 S)) <--> (reach_n H2 j) (env_locs rho2 S).
+  Proof.
+    intros Hres HB. split.
+    - intros l' [l [[m [Hm Hr]] Hin]].
+      eapply cc_approx_env_P_j_monotonic in Hres; eauto. 
+      eapply cc_approx_env_image_eq in Hres. eexists m.
+      split; eauto. eapply Hres. eexists. split; eauto.
+      eassumption.
+    - intros l' [m [Hm Hr]].
+      eapply cc_approx_env_P_j_monotonic in Hres; eauto. 
+      eapply cc_approx_env_image_eq in Hres. eapply Hres in Hr.
+      destruct Hr as [l [Heql Hin]]. eexists; split; eauto.
+      eexists; split; eauto. eassumption.
+  Qed.
+
+  Lemma cc_approx_env_image_reach GIP GP S (k : nat) (β : Inj)
+        (H1 H2 : heap block) (rho1 rho2 : env) :
+    (forall j, (H1, rho1) ⋞ ^ (S; k; j; GIP; GP; β) (H2, rho2)) ->
+    binding_in_map S rho1 ->
+    image β (reach' H1 (env_locs rho1 S)) <--> reach' H2 (env_locs rho2 S).
+  Proof.
+    intros Hres HB. split.
+    - intros l' [l [[m [Hm Hr]] Hin]].
+      eapply cc_approx_env_P_j_monotonic in Hres; eauto. 
+      eapply cc_approx_env_image_eq in Hres. eexists m.
+      split; eauto. eapply Hres. eexists. split; eauto.
+      eassumption.
+    - intros l' [m [Hm Hr]].
+      eapply cc_approx_env_P_j_monotonic in Hres; eauto. 
+      eapply cc_approx_env_image_eq in Hres. eapply Hres in Hr.
+      destruct Hr as [l [Heql Hin]]. eexists; split; eauto.
+      eexists; split; eauto. eassumption.
+  Qed.
+
+  (* TODO move *)
+
+  Lemma cc_approx_var_env_set_neq_r GIP GP b :
+    forall (k j : nat)  (rho1 rho2 : env) (H1 H2 : heap block)
+      (y1 x2 y2 : var) ( v2 : value),
+      cc_approx_var_env k j GIP GP b H1 rho1 H2 rho2 y1 y2 ->
+      y2 <> x2 ->
+      cc_approx_var_env k j GIP GP b H1 rho1 H2 (M.set x2 v2 rho2) y1 y2.
+  Proof. 
+    intros k j rho1 rho2 H1 H2 x2 y1 y2 v2 Hval Hneq x' Hget.
+    rewrite M.gso in *; eauto.
+  Qed.
+
+
+  Lemma project_var_preserves_cc_approx GII GI k j H1 rho1 H2 rho2 H2' rho2' b
+        Scope Funs σ c Γ FVs x x' C S S' m y y' :
+    project_var Scope Funs σ c Γ FVs S x x' C S' ->
+    cc_approx_var_env k j GII GI b H1 rho1 H2 rho2 y y' ->
+    ctx_to_heap_env C H2 rho2 H2' rho2' m ->
+    ~ y' \in S ->
+    cc_approx_var_env k j GII GI b H1 rho1 H2' rho2' y y'.
+  Proof.     
+    intros Hproj Hcc Hctx Hnin.
+    destruct Hproj; inv Hctx; eauto.
+    - inv H19. eapply cc_approx_var_env_set_neq_r; eauto.
+      intros Hc; subst; eauto.
+  Qed.
+
+  Lemma project_vars_preserves_cc_approx GII GI k j H1 rho1 H2 rho2 H2' rho2' b
+        Scope Funs σ c Γ FVs xs xs' C S S' m y y' :
+    project_vars Scope Funs σ c Γ FVs S xs xs' C S' ->
+    cc_approx_var_env k j GII GI b H1 rho1 H2 rho2 y y' ->
+    ctx_to_heap_env C H2 rho2 H2' rho2' m ->
+    ~ y' \in S ->
+    cc_approx_var_env k j GII GI b H1 rho1 H2' rho2' y y'.
+  Proof.     
+    intros Hvars. revert m H1 rho1 H2 rho2 H2' rho2'.
+    induction Hvars; intros m H1 rho1 H2 rho2 H2' rho2' Hcc Hctx Hnin.
+    - inv Hctx. eassumption.
+    - edestruct ctx_to_heap_env_comp_ctx_f_l as [rho3 [H3 [m1 [m2 [Hctx2 [Hctx3 Heq]]]]]]; eauto.
+      subst.
+      eapply IHHvars; [| eassumption | ].
+      eapply project_var_preserves_cc_approx; try eassumption.
+      intros Hc.
+      eapply Hnin. eapply project_var_free_set_Included; eauto.
+  Qed.  
+
+  (** Correctness of [project_var] *)
+  Lemma project_var_correct GII GI k  H1 rho1 H2 rho2 H2' rho2' b
+        Scope Funs σ c Γ FVs x x' C S S' m :
+    project_var Scope Funs σ c Γ FVs S x x' C S' ->
+    
+    (forall j, (H1, rho1) ⋞ ^ (Scope; k; j; GII; GI; b) (H2, rho2)) ->
+    (forall j, Fun_inv k j GII GI b rho1 H1 rho2 H2 Scope Funs σ) ->
+    (forall j, FV_inv k j GII GI b rho1 H1 rho2 H2 c Γ FVs) ->
+
+    ctx_to_heap_env C H2 rho2 H2' rho2' m ->
+
+    injective_subdomain (reach' H1 (env_locs rho1 (Scope :|: FromList FVs :|: Funs))) b ->
+    
+    binding_in_map Scope rho1 ->
+    Disjoint _ S (Scope :|: (image σ Funs) :|: (FromList FVs) :|: [set Γ]) ->
+
+    ~ In _ S' x' /\
+    injective_subdomain (reach' H1 (env_locs rho1 (x |: Scope :|: FromList FVs :|: Funs))) b /\
+    (forall j, (H1, rho1) ⋞ ^ (Scope; k; j; GII; GI; b) (H2', rho2'))  /\
+    (forall j, Fun_inv k j GII GI b rho1 H1 rho2' H2' Scope Funs σ) /\
+    (forall j, FV_inv k j GII GI b rho1 H1 rho2' H2' c Γ FVs) /\
+    (forall j, cc_approx_var_env k j GII GI b H1 rho1 H2' rho2' x x').
+  Proof with (now eauto with Ensembles_DB).
+    intros Hproj Hcc Hfun Henv Hctx Hinj Hbin Hd.
+    inv Hproj.
+    - inv Hctx. split. intros Hc. eapply Hd; eauto.
+      split; [| split; [| split ; [| split ]]]; eauto.
+      rewrite (Union_Same_set [set x'])... intros j; eapply Hcc. eassumption.
+    - inv Hctx.
+      split; [| split; [| split; [| split; [| split ]]]]. repeat split.
+      + intros Hc. eapply Hd. constructor; eauto.
+        left. left. right. eexists; split; eauto.
+      + rewrite <- !Union_assoc, (Union_commut [set x]), <- !Union_assoc, (Union_commut _ [set x]).
+        rewrite (Union_Same_set [set x]). rewrite !Union_assoc.  eassumption.
+        eapply Singleton_Included; eauto.
+      + intros j. eapply Hcc; eauto.
+      + eassumption.
+      + eassumption.
+      + intros j. edestruct (Hfun j) as (vf1 & vf2 & Hget1 & Hget2 & Hcc'); eauto.
+        intros v1 Hget1'. repeat subst_exp. eexists; split; eauto.
+    - inv Hctx. inv H19.
+      split; [| split; [| split; [| split; [| split ]]]]. repeat split.
+      + intros Hc. inv Hc. eauto.
+      + rewrite (Union_commut [set x]), <- (Union_assoc _ _ (FromList FVs)).
+        rewrite (Union_Same_set [set x]). eassumption.
+        eapply Singleton_Included; eauto. eapply nthN_In; eauto.
+      + intros j. eapply cc_approx_env_P_set_not_in_P_r. now eauto.
+        intros Hc. eapply Hd; eauto.
+      + intros j. eapply Fun_inv_set_not_in_Funs_r; eauto.
+        intros Hc; eapply Hd. constructor; eauto.
+      + intros h. 
+        edestruct Henv as (v1 & vs1 & l' & Hget1 & Hget2 & Hall).
+        repeat eexists; eauto. 
+        rewrite M.gso; eauto. intros Heq; subst. eapply Hd. constructor; eauto.
+      + intros j v' Hget.
+        edestruct (Henv j) as (v1 & vs1 & l' & Hget1 & Hget2 & Hall).
+        eexists. rewrite M.gss. split. reflexivity.
+        edestruct (Forall2_nthN _ FVs vs1 N _ Hall H3) as (v2 & Hnth' & vs4 & Hget4 & Hrel).
+        repeat subst_exp. eassumption.
+  Qed.
+
+  Lemma project_var_setminus_same  Scope Funs σ c Γ FVs x x' C S S' : 
+    project_var Scope Funs σ c Γ FVs S x x' C S' ->
+    project_var Scope (Funs \\ Scope) σ c Γ FVs S x x' C S'.
+  Proof. 
+    intros Hvar; destruct Hvar; try now constructor; eauto.
+    constructor; eauto. intros Hc; inv Hc; eauto.
+  Qed.
+
+  Lemma project_vars_setminus_same  Scope Funs σ c Γ FVs xs xs' C S S' : 
+    project_vars Scope Funs σ c Γ FVs S xs xs' C S' ->
+    project_vars Scope (Funs \\ Scope) σ c Γ FVs S xs xs' C S'.
+  Proof. 
+    intros Hvar; induction Hvar; try now constructor; eauto.
+    econstructor; eauto. eapply project_var_setminus_same. eassumption.
+  Qed.
+
+  (** Correctness of [project_vars] *)
+  Lemma project_vars_correct GII GI k  H1 rho1 H2 rho2 H2' rho2' b
+        Scope Funs σ c Γ FVs xs xs' C S S' m :
+    project_vars Scope Funs σ c Γ FVs S xs xs' C S' ->
+    
+    (forall j, (H1, rho1) ⋞ ^ (Scope; k; j; GII; GI; b) (H2, rho2)) ->
+    (forall j, Fun_inv k j GII GI b rho1 H1 rho2 H2 Scope Funs σ) ->
+    (forall j, FV_inv k j GII GI b rho1 H1 rho2 H2 c Γ FVs) ->
+
+    ctx_to_heap_env C H2 rho2 H2' rho2' m ->
+
+    injective_subdomain (reach' H1 (env_locs rho1 (Scope :|: FromList FVs :|: Funs))) b ->
+    
+    binding_in_map Scope rho1 -> 
+    Disjoint _ S (Scope :|: (image σ Funs) :|: (FromList FVs) :|: [set Γ]) ->
+
+    Disjoint _ (FromList xs') S' /\
+    injective_subdomain (reach' H1 (env_locs rho1 ((FromList xs) :|: Scope :|: FromList FVs :|: Funs))) b /\
+    (forall j, (H1, rho1) ⋞ ^ (Scope; k; j; GII; GI; b) (H2', rho2'))  /\
+    (forall j, Fun_inv k j GII GI b rho1 H1 rho2' H2' Scope Funs σ) /\
+    (forall j, FV_inv k j GII GI b rho1 H1 rho2' H2' c Γ FVs) /\
+    (forall j, Forall2 (fun x x' => cc_approx_var_env k j GII GI b H1 rho1 H2' rho2' x x') xs xs').
+  Proof with (now eauto with Ensembles_DB).
+    intros Hvars. revert m H1 rho1 H2 rho2 H2' rho2'.
+    induction Hvars; intros m H1 rho1 H2 rho2 H2' rho2' Hcc Hfun Hfv Hctx Hinj Hb Hd. 
+    - inv Hctx. split; [| split; [| split ; [| split ]]]; eauto.
+      rewrite FromList_nil...
+      rewrite FromList_nil. rewrite Union_Empty_set_neut_l...
+    - rewrite FromList_cons in *. 
+      edestruct ctx_to_heap_env_comp_ctx_f_l as [rho3 [H3 [m1 [m2 [Hctx2 [Hctx3 Heq]]]]]].
+      subst.
+      eassumption. subst.
+      edestruct project_var_correct as (Hd' & Hinj' & Hcc' & Hfun' & Hfv' & Hall');
+        try eassumption.
+      edestruct IHHvars as (Hd'' & Hinj'' & Hcc'' & Hfun'' & Hfv'' & Hall'');
+      try eassumption.
+      eapply Disjoint_Included_l; [| eassumption ].
+      eapply project_var_free_set_Included. eassumption.
+      split; [| split; [| split ; [| split; [| split ] ]]]; eauto.
+      * eapply Union_Disjoint_l. 
+        eapply Disjoint_Included_r.
+        eapply project_vars_free_set_Included. eassumption.
+        eapply Disjoint_Singleton_l.
+        eapply project_var_not_In_free_set. eassumption.
+        eapply Disjoint_Included_r; [| eassumption ].
+        rewrite <- !Union_assoc. eapply Included_Union_compat. reflexivity.
+        eapply Included_Union_compat. eapply image_monotonic...
+        reflexivity.        
+        eapply Disjoint_sym. eapply project_vars_not_In_free_set. eassumption.
+        eapply Disjoint_Included_l.
+        eapply project_var_free_set_Included. eassumption.
+        eapply Disjoint_Included_r; [| eassumption ].
+        rewrite <- !Union_assoc. eapply Included_Union_compat. reflexivity.
+        eapply Included_Union_compat. eapply image_monotonic...
+        reflexivity.
+      * eapply injective_subdomain_antimon. now apply Hinj.
+        eapply reach'_set_monotonic. eapply env_locs_monotonic.
+        rewrite FromList_cons. rewrite <- !Union_assoc. eapply Union_Included.
+        eapply Singleton_Included. rewrite (Union_commut (FromList FVs)).
+        eapply project_var_In_Union. eassumption.
+        eapply Union_Included.  rewrite (Union_commut (FromList FVs)).
+        eapply project_vars_In_Union. eassumption.
+        now eauto with Ensembles_DB.
+      * intros j. constructor; eauto .
+        eapply project_vars_preserves_cc_approx; eauto.
+  Qed.
+  
+
   (** Correctness of [Closure_conversion] *)
   Lemma Closure_conversion_correct (k : nat) (H1 H2 : heap block)
         (rho1 rho2 : env) (e1 e2 : exp) (C : exp_ctx)
@@ -538,28 +1059,30 @@ Module ClosureConversionCorrect (H : Heap).
     (* [Scope] invariant *)
     (forall j, (H1, rho1) ⋞ ^ (Scope ; k ; j ; Pre Hole_c ; Post 0 ; β) (H2, rho2)) ->
     (* [Fun] invariant *)
-    Fun_inv k (Pre Hole_c) (Post 0) β rho1 H1 rho2 H2 Scope Funs σ c Γ ->
+    (forall j, Fun_inv k j (Pre Hole_c) (Post 0) β rho1 H1 rho2 H2 Scope Funs σ) ->
     (* Free variables invariant *)
-    FV_inv k (Pre Hole_c) (Post 0) β rho1 H1 rho2 H2 Scope Funs c Γ FVs ->
+    (forall j, FV_inv k j (Pre Hole_c) (Post 0) β rho1 H1 rho2 H2 c Γ FVs) ->
     (* location renaming is injective *)
-    injective_subdomain (reach H1 (env_locs rho1 Scope)) β ->
+    (* only needed to prove the lower bound *)
+    injective_subdomain (reach' H1 (env_locs rho1 (Scope :|: FromList FVs :|: Funs))) β ->
     
     (* well-formedness *)
-    well_formed (reach' H1 (env_locs rho1 (occurs_free e1))) H1 ->
-    (env_locs rho1 (occurs_free e1)) \subset dom H1 ->
-    well_formed (reach' H2 (env_locs rho2 (occurs_free (C |[ e2 ]|)))) H2 ->
-    (env_locs rho2 (occurs_free (C |[ e2 ]|))) \subset dom H2 ->
+    well_formed (reach' H1 (env_locs rho1 (Scope :|: Funs :|: FromList FVs))) H1 ->
+    (env_locs rho1 (Scope :|: Funs :|: FromList FVs)) \subset dom H1 ->
+    well_formed (reach' H2 (env_locs rho2 (Scope :|: (image σ Funs) :|: [set Γ]))) H2 ->
+    (env_locs rho2 (Scope :|:  (image σ Funs) :|: [set Γ])) \subset dom H2 ->
 
+    
     (* [Γ] (the current environment parameter) is not bound in e *)
     ~ In _ (bound_var e1) Γ ->
     (* The free variables of e are defined in the environment *)
-    binding_in_map (occurs_free e1) rho1 ->
+    binding_in_map (Scope :|: Funs :|: FromList FVs) rho1 ->
     (* The blocks of functions have unique function names *)
     fundefs_names_unique e1 ->
     (* function renaming is injective in the [Funs] subdomain *)
     injective_subdomain Funs σ ->
     (* function renaming codomain is not shadowed by other vars *)
-    Disjoint _ (image σ (Setminus _ Funs Scope)) (bound_var e1) ->
+    Disjoint _ (image σ Funs) (bound_var e1) ->
 
     
     (* [e'] is the closure conversion of [e] *)
@@ -573,98 +1096,245 @@ Module ClosureConversionCorrect (H : Heap).
            Henv Hfun HFVs Hinjb Hwf1 Hlocs1 Hwf2 Hlocs2 Hnin Hbind Hun Hinj Hd Hcc.
     induction e1 using exp_ind'; try clear IHe1.
     - (* case Econstr *)
+      assert (Hfv := Closure_conversion_pre_occurs_free_Included _ _ _ _ _ _ _ _ _ _ Hcc).
+      assert (Hfv' := Closure_conversion_occurs_free_Included _ _ _ _ _ _ _ _ _ _ Hcc Hun).
+      rewrite !Union_assoc in Hfv'.
+
       inv Hcc.
-      
       edestruct (binding_in_map_getlist _ rho1 l Hbind) as [vl Hgetl].
-      normalize_occurs_free...
+      rewrite <- Union_assoc. eapply project_vars_In_Union. eassumption.
       
       edestruct project_vars_ctx_to_heap_env as [H2' [rho2' [m Hct]]]; try eassumption.
-      eapply Fun_inv_weak_in_Fun_inv; eassumption.
-      eapply FV_inv_weak_in_FV_inv; eassumption.
-
+      specialize (Hfun 0); eapply Fun_inv_weak_in_Fun_inv; eassumption.
+      specialize (HFVs 0); eapply FV_inv_weak_in_FV_inv; eassumption.
+      
       intros j.
       (* process right ctx *)
       eapply cc_approx_exp_right_ctx_compat
       with (ILi := fun c => PostL c k H1 rho1 (Econstr v t l e1)) (II := fun C => Pre C k);
         [ now intros; eapply Post_transfer; eauto | now intros; eapply IP_ctx_to_heap_env; eauto
-          | eassumption | eassumption | eassumption | eassumption | eassumption | ].
+          | | | | | eassumption | ].
+
+      eapply well_formed_antimon. eapply reach'_set_monotonic. now eapply env_locs_monotonic; eauto.
+      eassumption.
+
+      eapply well_formed_antimon. eapply reach'_set_monotonic. now eapply env_locs_monotonic; eauto.
+      eassumption.
+
+      eapply Included_trans; [| eassumption ]. now eapply env_locs_monotonic; eauto.
+      eapply Included_trans; [| eassumption ]. eapply env_locs_monotonic; eauto.
+      
       rewrite <- plus_n_O.
       replace (comp_ctx_f Hole_c C) with C by eauto.
       assert (Hwf2' := Hwf2).
       assert (Hlocs2' := Hlocs2). 
-      eapply project_vars_well_formed in Hwf2; try eassumption.
-      eapply project_vars_env_locs in Hlocs2; try eassumption.
+      eapply project_vars_well_formed' in Hwf2; try eassumption.
+      eapply project_vars_env_locs' in Hlocs2; try eassumption.
+
+      edestruct project_vars_correct as (Hd' & Hinj' & Henv' & Hfun' & HFVs' & Hvars);
+        try eassumption.
+      eapply binding_in_map_antimon; [| eassumption ]...
+      rewrite <- !Union_assoc. eassumption.
+      
       (* process Econstr one the right and left *)
       eapply cc_approx_exp_constr_compat 
       with (ILi := fun c => PostL c k H1 rho1 (Econstr v t l e1))
            (r2 := 0)
            (IIL2 := Pre Hole_c (k - cost H1 rho1 (Econstr v t l e1)));
-        [ | | | eassumption | eassumption | eassumption  | eassumption | | | ]. 
+        [ | | | | | | | eassumption | | ]. 
       + admit. (* bounds timeout compat *)
       + admit. (* bounds - pick F *)
       + admit. (* pre - allocation *) (* TODO maybe we need less assumptions *)
-      + admit. (* project_vars_correct *)
+      + eapply well_formed_antimon; [| eassumption ].
+        eapply reach'_set_monotonic. eapply env_locs_monotonic. eassumption.
+      + eapply project_vars_well_formed; eauto.
+        eapply Included_trans; [| eassumption ]. eapply env_locs_monotonic.
+        eassumption. eapply well_formed_antimon; [| eassumption ].
+        eapply reach'_set_monotonic. eapply env_locs_monotonic. eassumption.
+      + eapply Included_trans; [| eassumption ]. eapply env_locs_monotonic.
+        eassumption.
+      + eapply project_vars_env_locs; eauto. eapply Included_trans. 
+        eapply env_locs_monotonic. eassumption. eassumption.
+        eapply well_formed_antimon.
+        eapply reach'_set_monotonic. eapply env_locs_monotonic. eassumption.
+        eassumption.
       + admit. (* bounds -- find F *)
       + (* Inductive case *) 
         intros vs1 vs2 l1 l2 H1' H2'' Hleq Ha1 Ha2 Hr1 Hr2 Hall j1.
         (* monotonicity of the local invariant *)
-        eapply cc_approx_exp_rel_mon with (LP1 := PostL 0 (k - cost H1 rho1 (Econstr v t l e1)) H1' (M.set v (Loc l1) rho1) e1). 
+        eapply cc_approx_exp_rel_mon
+        with (LP1 := PostL 0 (k - cost H1 rho1 (Econstr v t l e1)) H1' (M.set v (Loc l1) rho1) e1).
         
         (* Induction hypothesis *)
-        {  eapply IHk;
-          [ | | | | | | | | | | | | eassumption | | eassumption ].
+        { eapply IHk;
+          [ | | | | | | | | | | | | now apply Hinj | | eassumption ]. 
           * simpl in *. omega.
-          * intros j2.
-            eapply cc_approx_env_set_alloc_Constr with (b := β {l1 ~> l2}); try eassumption.
-            admit.
-            admit.
-            admit.
-            admit.
-            admit.
-            admit.
-            admit.
-            (* eapply cc_approx_env_P_antimon. *)
-            rewrite extend_gss. reflexivity.
-            intros j3 Hlt3. eapply Forall2_monotonic_strong; [| now eapply Hall ].
-            intros x1 x2 Hin1 Hin2 Hrel. eapply cc_approx_val_rename_ext. now eapply Hrel.
-            eapply f_eq_subdomain_extend_not_In_S_l; [| reflexivity ].
-            intros Hc. eapply reachable_in_dom in Hc.
-            destruct Hc as [v1 Hgetv1]. erewrite alloc_fresh in Hgetv1; try eassumption. congruence.
-            eapply well_formed_antimon; [| eassumption ].
-            eapply reach'_set_monotonic. eapply Included_trans; [| eassumption ].
-            simpl. eapply In_Union_list. eapply in_map. eassumption.
-            eapply Included_trans; [| eassumption ].
-            eapply Included_trans; [| eassumption ].
-            simpl. eapply In_Union_list. eapply in_map. eassumption.
+          * { intros j2.  
+              eapply cc_approx_env_set_alloc_Constr with (b := β {l1 ~> l2});
+                try eassumption.
+              - eapply well_formed_antimon; [| eassumption ].
+                eapply reach'_set_monotonic. eapply env_locs_monotonic...
+              - eapply well_formed_antimon; [| eassumption ].
+                eapply reach'_set_monotonic. eapply env_locs_monotonic.
+                now eauto 20 with Ensembles_DB.
+              - eapply Included_trans; [| eassumption ].
+                eapply env_locs_monotonic...
+              - eapply Included_trans; [| eassumption ].
+                eapply env_locs_monotonic.
+                now eauto 20 with Ensembles_DB.
+              - eapply well_formed_antimon. eapply reach'_set_monotonic.
+                eassumption.
+                eapply well_formed_antimon; [| eassumption ].
+                eapply reach'_set_monotonic. eapply env_locs_monotonic...
+              - eapply well_formed_antimon. eapply reach'_set_monotonic.
+                eassumption.
+                eapply project_vars_well_formed; eauto.
+                eapply Included_trans; [| eassumption ]. eapply env_locs_monotonic.
+                eassumption. eapply well_formed_antimon; [| eassumption ].
+                eapply reach'_set_monotonic. eapply env_locs_monotonic. eassumption.
+              - eapply Included_trans. eassumption.
+                eapply Included_trans; [| eassumption ].
+                eapply env_locs_monotonic...
+              - eapply Included_trans. eassumption.
+                eapply project_vars_env_locs; eauto. eapply Included_trans. 
+                eapply env_locs_monotonic. eassumption. eassumption.
+                eapply well_formed_antimon.
+                eapply reach'_set_monotonic. eapply env_locs_monotonic. eassumption.
+                eassumption.
+              - eapply cc_approx_env_rename_ext.
+                eapply cc_approx_env_P_antimon.
+                eapply cc_approx_env_P_monotonic. now eauto.
+                simpl in *; omega. now eauto with Ensembles_DB.
+                eapply f_eq_subdomain_extend_not_In_S_r; [| reflexivity ].
+                intros Hc. eapply reachable_in_dom in Hc.
+                edestruct Hc as [vc Hgetc]. erewrite alloc_fresh in Hgetc; eauto. congruence.
+                eapply well_formed_antimon; [| eassumption ].
+                eapply reach'_set_monotonic. eapply env_locs_monotonic...
+                eapply Included_trans; [| eassumption ]. eapply env_locs_monotonic...
+              - rewrite extend_gss. reflexivity.
+              - intros j3 Hlt3. eapply Forall2_monotonic_strong; [| now eapply Hall ].
+                intros x1 x2 Hin1 Hin2 Hrel. eapply cc_approx_val_rename_ext. now eapply Hrel.
+                assert (Hincl : val_loc x1 \subset env_locs rho1 (Scope :|: Funs :|: FromList FVs)).
+                { eapply Included_trans; [| now eapply env_locs_monotonic; eauto ].
+                  eapply Included_trans; [| eassumption ].
+                  simpl. eapply In_Union_list. eapply in_map. eassumption. }
+                
+                eapply f_eq_subdomain_extend_not_In_S_l; [| reflexivity ].
+                
+                intros Hc. eapply reachable_in_dom in Hc.
+                destruct Hc as [v1 Hgetv1]. erewrite alloc_fresh in Hgetv1; try eassumption.
+                congruence.
+                
+                eapply well_formed_antimon; [| eassumption ].
+                eapply reach'_set_monotonic. eassumption.
+
+                eapply Included_trans; eassumption. }
           * admit. (* fun inv env_set_alloc *)
           * admit. (* FV inv env set alloc *)
-          * eapply injective_subdomain_extend'. admit. admit.
-          * eapply well_formed_antimon;
-            [| rewrite occurs_free_Econstr in Hwf1;
-               eapply well_formed_reach_alloc'; try eassumption ]. 
-            eapply reach'_set_monotonic. eapply env_locs_monotonic...
-            eapply Included_trans; [| eassumption ]. normalize_occurs_free...
-            rewrite env_locs_Union. eapply Included_trans. eassumption.
-            normalize_occurs_free. rewrite env_locs_Union...
+          * assert
+              (Hinc :
+                 reach' H1'
+                        (env_locs (M.set v (Loc l1) rho1)
+                                  (v |: Scope :|: FromList FVs :|: Funs)) \\ [set l1]
+                        \subset
+                  reach' H1 (env_locs rho1 (Scope :|: FromList FVs :|: Funs))
+              ).
+            { eapply Included_trans. eapply Included_Setminus_compat.
+              eapply Included_trans;
+                [| eapply reach'_alloc_set with (H' := H1')
+                                                (S := Scope :|: FromList FVs :|: Funs)];
+              try eassumption.
+              eapply reach'_set_monotonic. eapply env_locs_monotonic.
+              now eauto 20 with Ensembles_DB.
+              eapply Included_trans. eassumption.
+              eapply Included_trans; [| eapply reach'_extensive ].
+              eapply env_locs_monotonic. eapply Included_trans; [ eassumption |]...
+              reflexivity. 
+              rewrite Setminus_Union_distr, Setminus_Same_set_Empty_set,
+              Union_Empty_set_neut_l.
+              eapply Setminus_Included_preserv.
+              eapply reach'_set_monotonic. eapply env_locs_monotonic.
+              now eauto 20 with Ensembles_DB. }
+            eapply injective_subdomain_extend'.
+            { eapply injective_subdomain_antimon. eassumption.
+              eapply Included_trans. eassumption.
+              eapply reach'_set_monotonic. eapply env_locs_monotonic.
+              now eauto 20 with Ensembles_DB. }
+            { intros Hc. eapply image_monotonic in Hc; [| eassumption ].
+              rewrite !env_locs_Union, !reach'_Union, !image_Union in Hc.
+              rewrite cc_approx_env_image_reach in Hc; try eassumption. 
+              rewrite FV_inv_image_reach in Hc; try eassumption.
+              rewrite Fun_inv_image_reach in Hc; try eassumption.
+              rewrite <- !reach'_Union in Hc. eapply reachable_in_dom in Hc.
+              destruct Hc as [vc Hgetc]. erewrite alloc_fresh in Hgetc; eauto. congruence.
+              eapply well_formed_antimon; [| eassumption ].
+              rewrite !env_locs_Union, !reach'_Union.
+              rewrite <- !Union_assoc. eapply Included_Union_preserv_r.
+              eapply Included_Union_compat. reflexivity. rewrite Union_commut.
+              eapply Included_Union_compat. reflexivity.
+              rewrite (reach_unfold H2' (env_locs _ _))...
+              eapply Union_Included. eapply Union_Included.
+              eapply Included_trans; [| eassumption ]. eapply env_locs_monotonic...
+              eapply Included_trans; [| eapply reachable_in_dom; eauto ].
+              rewrite !env_locs_Union, !reach'_Union.
+              eapply Included_Union_preserv_r. eapply Included_post_reach'.
+              eapply Included_trans; [| eassumption ]. eapply env_locs_monotonic...
+              eapply binding_in_map_antimon; [| eassumption ]... }
+          * assert (Hseq : v |: Scope :|: Funs :|: FromList FVs <-->
+                             (Scope :|: Funs :|: FromList FVs) :|: [set v]).
+            { rewrite (Union_commut _ [set v]). rewrite <- !Union_assoc. reflexivity. }
+            rewrite Hseq. eapply well_formed_reach_alloc'; try eassumption.
+            rewrite Setminus_Same_set_Empty_set, Union_Empty_set_neut_r.
+            eassumption.
+            rewrite Setminus_Same_set_Empty_set, Union_Empty_set_neut_r.
+            eassumption.
+            rewrite Setminus_Same_set_Empty_set, Union_Empty_set_neut_r.
+            eapply Included_trans. eassumption.
+            eapply Included_trans; [| eapply reach'_extensive ].
+            eapply env_locs_monotonic. eassumption.
           * eapply Included_trans. now eapply env_locs_set_Inlcuded'.
             rewrite HL.alloc_dom; [| eassumption ].
             eapply Included_Union_compat. reflexivity.
             eapply Included_trans; [| eassumption ].
-            normalize_occurs_free...
-          * eapply well_formed_antimon;
+            eapply env_locs_monotonic. now eauto 20 with Ensembles_DB.
+          * assert (Hseq : v |: Scope :|: image σ Funs :|: [set Γ] <-->
+                             (Scope :|: image σ Funs :|: [set Γ]) :|: [set v]).
+            { rewrite (Union_commut _ [set v]). rewrite <- !Union_assoc. reflexivity. }
+            rewrite Hseq. eapply well_formed_reach_set_Loc. 
+            rewrite Hseq. eapply well_formed_reach_alloc'; try eassumption.
+            rewrite Setminus_Same_set_Empty_set, Union_Empty_set_neut_r.
+            eapply well_formed_antimon; [| eassumption ].
+            eapply reach'_set_monotonic. eapply env_locs_monotonic...
+            rewrite Setminus_Same_set_Empty_set, Union_Empty_set_neut_r.
+            eapply Included_trans; [| eassumption ].
+            eapply env_locs_monotonic...
+            eapply Included_trans. eassumption. 
+            eapply Included_trans. eapply project_vars_env_locs. eassumption. eassumption.
+            eapply Included_trans. eapply env_locs_monotonic. eassumption.
+            eassumption.
+            eapply well_formed_antimon; [| eassumption ].
+            eapply reach'_set_monotonic. eapply env_locs_monotonic. eassumption.
+            
+            eapply Closure_conversion_occurs_free_Included. eassumption. eapply reach'_set_monotonic. eapply env_locs_monotonic...
+            [| eassumption ].
+            eapply env_locs_monotonic...
+            Scope :|: image σ Funs :|: [set Γ
+            eapply Included_trans; [| 
+            eassumption. 
+            eapply well_formed_antimon;
             [| rewrite occurs_free_Econstr in Hwf2;
                eapply well_formed_reach_alloc'; try eassumption ]. 
             eapply reach'_set_monotonic. eapply env_locs_monotonic...
             eapply Included_trans; [| eassumption ]. normalize_occurs_free...
-            rewrite env_locs_Union. eapply Included_trans. eassumption.
-            normalize_occurs_free. rewrite env_locs_Union...
+            eapply Included_trans. eassumption.
+            normalize_occurs_free. eapply reach'_extensive.
           * eapply Included_trans. now eapply env_locs_set_Inlcuded'.
             rewrite HL.alloc_dom; [| eassumption ].
             eapply Included_Union_compat. reflexivity.
             eapply Included_trans; [| eassumption ]. normalize_occurs_free...
           * now eauto.
           * eapply binding_in_map_antimon; [| eapply binding_in_map_set; eassumption ].
-            eapply occurs_free_Econstr_Included.
+            now eauto 20 with Ensembles_DB.
           * intros f Hfin. eauto.
           * eapply Disjoint_Included_r;
               [| eapply Disjoint_Included_l; [ apply image_monotonic | now apply Hd ]].
